prove GLAE

raft-proofs/GhostLogAllEntriesProof.v
@@ -11,6 +11,7 @@ Require Import CommonDefinitions.
 Require Import CommonTheorems.
 Require Import SpecLemmas.
 Require Import RefinementSpecLemmas.
+Require Import RaftRefinementInterface.
 Require Import RaftMsgRefinementInterface.
 
 Require Import InLogInAllEntriesInterface.
@@ -40,8 +41,255 @@ Section GhostLogAllEntriesProof.
 
   Ltac destruct_update :=
     repeat (first [update_destruct_hyp|update_destruct]; subst; rewrite_update).
+
+  Definition lifted_in_log_in_all_entries (net : network) :=
+    forall h e,
+      In e (log (snd (nwState net h))) ->
+      exists t,
+        In (t, e) (allEntries (fst (nwState net h))).
+
+  Lemma lifted_in_log_in_all_entries_invariant :
+    forall (net : @network _ raft_msg_refined_multi_params),
+      msg_refined_raft_intermediate_reachable net ->
+      lifted_in_log_in_all_entries net.
+  Proof.
+    intros.
+    unfold lifted_in_log_in_all_entries; intros.
+    find_eapply_lem_hyp msg_lift_prop;
+      [|intros; eapply in_log_in_all_entries_invariant; eauto].
+    simpl in *.
+    unfold in_log_in_all_entries in *.
+    unfold mgv_deghost in *.
+    simpl in *.
+    repeat break_match; simpl in *; eauto.
+  Qed.
+
+  Lemma update_elections_data_appendEntries_preserves_allEntries' :
+    forall st h t n pli plt es ci x,
+      In x (allEntries (fst st)) ->
+      In x (allEntries (update_elections_data_appendEntries h st t n pli plt es ci)).
+  Proof.
+    unfold update_elections_data_appendEntries.
+    intros. break_let. break_match; auto.
+    break_if; auto.
+    simpl. intuition.
+  Qed.
+
+  Lemma ghost_log_allEntries_append_entries :
+    msg_refined_raft_net_invariant_append_entries ghost_log_allEntries.
+  Proof.
+    red. unfold ghost_log_allEntries. intros. simpl in *.
+    subst. repeat find_higher_order_rewrite.
+    destruct_update; simpl in *; eauto.
+    - repeat find_rewrite.
+      find_apply_hyp_hyp; intuition; eauto.
+      + eapply_prop_hyp In In; eauto.
+        break_exists_exists.
+        eauto using update_elections_data_appendEntries_preserves_allEntries'.
+      + remember (pSrc p0).
+        subst. simpl in *.
+        unfold write_ghost_log in *.
+        find_eapply_lem_hyp lifted_in_log_in_all_entries_invariant; eauto.
+        break_exists_exists.
+        eauto using update_elections_data_appendEntries_preserves_allEntries'.
+    - find_apply_hyp_hyp; intuition; eauto.
+      subst. simpl in *.
+      unfold write_ghost_log in *.
+      eapply lifted_in_log_in_all_entries_invariant; eauto.
+  Qed.
+
+  Lemma ghost_log_allEntries_append_entries_reply :
+    msg_refined_raft_net_invariant_append_entries_reply ghost_log_allEntries.
+  Proof.
+    red. unfold ghost_log_allEntries. intros. simpl in *.
+    subst. repeat find_higher_order_rewrite.
+    destruct_update; simpl in *; eauto.
+    - find_apply_hyp_hyp; intuition; eauto.
+      + eapply_prop_hyp In In;
+        repeat find_rewrite; eauto.
+      + do_in_map.
+        subst. simpl in *. unfold add_ghost_msg in *.
+        do_in_map. subst. simpl in *. unfold write_ghost_log in *.
+        eapply lifted_in_log_in_all_entries_invariant; eauto.
+    - find_apply_hyp_hyp; intuition; eauto.
+      do_in_map.
+      subst. simpl in *. unfold add_ghost_msg in *.
+      do_in_map. subst. simpl in *. unfold write_ghost_log in *.
+      eapply lifted_in_log_in_all_entries_invariant; eauto.
+  Qed.
+
+  Lemma ghost_log_allEntries_request_vote :
+    msg_refined_raft_net_invariant_request_vote ghost_log_allEntries.
+  Proof.
+    red. unfold ghost_log_allEntries. intros. simpl in *.
+    subst. repeat find_higher_order_rewrite.
+    destruct_update; simpl in *; eauto.
+    - rewrite update_elections_data_requestVote_allEntries.
+      find_apply_hyp_hyp; intuition; eauto.
+      + eapply_prop_hyp In In;
+        repeat find_rewrite; eauto.
+      + subst. simpl in *. unfold write_ghost_log in *.
+        eapply lifted_in_log_in_all_entries_invariant; eauto.
+    - find_apply_hyp_hyp; intuition; eauto.
+      subst. simpl in *. unfold write_ghost_log in *.
+      eapply lifted_in_log_in_all_entries_invariant; eauto.
+  Qed.
+
+  Lemma ghost_log_allEntries_request_vote_reply :
+    msg_refined_raft_net_invariant_request_vote_reply ghost_log_allEntries.
+  Proof.
+    red. unfold ghost_log_allEntries. intros. simpl in *.
+    subst. repeat find_higher_order_rewrite.
+    destruct_update; simpl in *; eauto.
+    rewrite update_elections_data_requestVoteReply_allEntries.
+    repeat find_rewrite.
+    find_apply_hyp_hyp.
+    eauto.
+  Qed.
+
+  Lemma ghost_log_allEntries_timeout :
+    msg_refined_raft_net_invariant_timeout ghost_log_allEntries.
+  Proof.
+    red. unfold ghost_log_allEntries. intros. simpl in *.
+    subst. repeat find_higher_order_rewrite.
+    destruct_update; simpl in *; eauto.
+    - rewrite update_elections_data_timeout_allEntries.
+      find_apply_hyp_hyp; intuition; eauto.
+      do_in_map.
+      remember (pSrc p).
+      subst p. simpl in *. unfold add_ghost_msg in *.
+      do_in_map. subst. simpl in *. unfold write_ghost_log in *.
+      eapply lifted_in_log_in_all_entries_invariant; eauto.
+    - find_apply_hyp_hyp; intuition; eauto.
+      do_in_map.
+      remember (pSrc p).
+      subst p. simpl in *. unfold add_ghost_msg in *.
+      do_in_map. subst. simpl in *. unfold write_ghost_log in *.
+      eapply lifted_in_log_in_all_entries_invariant; eauto.
+  Qed.
+
+  Lemma ghost_log_allEntries_client_request :
+    msg_refined_raft_net_invariant_client_request ghost_log_allEntries.
+  Proof.
+    red. unfold ghost_log_allEntries. intros. simpl in *.
+    subst. repeat find_higher_order_rewrite.
+    destruct_update; simpl in *; eauto.
+    - enough (exists t, In (t, e) (allEntries (fst (nwState net (pSrc p))))) by
+          (break_exists_exists;
+           eauto using update_elections_data_clientRequest_allEntries_old').
+      find_apply_hyp_hyp; intuition; eauto.
+      do_in_map.
+      remember (pSrc p).
+      subst p. simpl in *. unfold add_ghost_msg in *.
+      do_in_map. subst. simpl in *. unfold write_ghost_log in *.
+      eapply lifted_in_log_in_all_entries_invariant; eauto.
+    - find_apply_hyp_hyp; intuition; eauto.
+      do_in_map.
+      remember (pSrc p).
+      subst p. simpl in *. unfold add_ghost_msg in *.
+      do_in_map. subst. simpl in *. unfold write_ghost_log in *.
+      eapply lifted_in_log_in_all_entries_invariant; eauto.
+  Qed.
+
+  Lemma ghost_log_allEntries_do_leader :
+    msg_refined_raft_net_invariant_do_leader ghost_log_allEntries.
+  Proof.
+    red. unfold ghost_log_allEntries. intros. simpl in *.
+    match goal with
+      | H : nwState ?net ?h = (?gd, ?d) |- _ =>
+        replace gd with (fst (nwState net h)) in * by (rewrite H; reflexivity);
+          replace d with (snd (nwState net h)) in * by (rewrite H; reflexivity);
+          clear H
+    end.
+    subst. repeat find_higher_order_rewrite.
+    destruct_update; simpl in *; eauto.
+    - find_apply_hyp_hyp; intuition; eauto.
+      do_in_map.
+      remember (pSrc p).
+      subst p. simpl in *. unfold add_ghost_msg in *.
+      do_in_map. subst. simpl in *. unfold write_ghost_log in *.
+      eapply lifted_in_log_in_all_entries_invariant; eauto.
+    - find_apply_hyp_hyp; intuition; eauto.
+      do_in_map.
+      remember (pSrc p).
+      subst p. simpl in *. unfold add_ghost_msg in *.
+      do_in_map. subst. simpl in *. unfold write_ghost_log in *.
+      eapply lifted_in_log_in_all_entries_invariant; eauto.
+  Qed.
+
+  Lemma ghost_log_allEntries_do_generic_server :
+    msg_refined_raft_net_invariant_do_generic_server ghost_log_allEntries.
+  Proof.
+    red. unfold ghost_log_allEntries. intros. simpl in *.
+    match goal with
+      | H : nwState ?net ?h = (?gd, ?d) |- _ =>
+        replace gd with (fst (nwState net h)) in * by (rewrite H; reflexivity);
+          replace d with (snd (nwState net h)) in * by (rewrite H; reflexivity);
+          clear H
+    end.
+    subst. repeat find_higher_order_rewrite.
+    destruct_update; simpl in *; eauto.
+    - find_apply_hyp_hyp; intuition; eauto.
+      do_in_map.
+      remember (pSrc p).
+      subst p. simpl in *. unfold add_ghost_msg in *.
+      do_in_map. subst. simpl in *. unfold write_ghost_log in *.
+      eapply lifted_in_log_in_all_entries_invariant; eauto.
+    - find_apply_hyp_hyp; intuition; eauto.
+      do_in_map.
+      remember (pSrc p).
+      subst p. simpl in *. unfold add_ghost_msg in *.
+      do_in_map. subst. simpl in *. unfold write_ghost_log in *.
+      eapply lifted_in_log_in_all_entries_invariant; eauto.
+  Qed.
+
+  Lemma ghost_log_allEntries_reboot :
+    msg_refined_raft_net_invariant_reboot ghost_log_allEntries.
+  Proof.
+    red. unfold ghost_log_allEntries. intros. simpl in *.
+    match goal with
+      | H : nwState ?net ?h = (?gd, ?d) |- _ =>
+        replace gd with (fst (nwState net h)) in * by (rewrite H; reflexivity);
+          replace d with (snd (nwState net h)) in * by (rewrite H; reflexivity);
+          clear H
+    end.
+    subst. repeat find_higher_order_rewrite.
+    destruct_update; simpl in *; eauto.
+  Qed.
+  
+  Lemma ghost_log_allEntries_state_same_packet_subset :
+    msg_refined_raft_net_invariant_state_same_packet_subset ghost_log_allEntries.
+  Proof.
+    red. unfold ghost_log_allEntries. intros. simpl in *.
+    subst. repeat find_higher_order_rewrite.
+    destruct_update; simpl in *; eauto.
+    find_apply_hyp_hyp.
+    repeat find_reverse_higher_order_rewrite.
+    eauto.
+  Qed.
+  
+  Lemma ghost_log_allEntries_init :
+    msg_refined_raft_net_invariant_init ghost_log_allEntries.
+  Proof.
+    red. unfold ghost_log_allEntries. intros. simpl in *.
+    intuition.
+  Qed.
   
   Instance glaei : ghost_log_allEntries_interface.
   Proof.
-  Admitted.
+    split.
+    intros.
+    apply msg_refined_raft_net_invariant; auto.
+    - apply ghost_log_allEntries_init.
+    - apply ghost_log_allEntries_client_request.
+    - apply ghost_log_allEntries_timeout.
+    - apply ghost_log_allEntries_append_entries.
+    - apply ghost_log_allEntries_append_entries_reply.
+    - apply ghost_log_allEntries_request_vote.
+    - apply ghost_log_allEntries_request_vote_reply.
+    - apply ghost_log_allEntries_do_leader.
+    - apply ghost_log_allEntries_do_generic_server.
+    - apply ghost_log_allEntries_state_same_packet_subset.
+    - apply ghost_log_allEntries_reboot.
+  Qed.
 End GhostLogAllEntriesProof.
